hol/bdd_gen_correctScript.sml
@@ -29,12 +29,46 @@ val _ = new_theory "bdd_gen_correct";
 
 
 
+(* TODO: figure out how to put all of those in one file *)
+    
+val body_of_mk_pred_tac =    
+( rename1 ‘getLeaves edges r = SOME leaves’ >>
+  rename1 ‘getLabels labels leaves = SOME leaves_labels’ >>
+  rename1 ‘extract_nontermn leaves_labels = SOME ntl’ >>
+  
+  ‘∃ leaves_sub . leaves_pred_sub rec ntl h = leaves_sub’ by gvs[] >>
+  ‘∃ simp_leaves . simp_pred_list rec leaves_sub = simp_leaves’ by gvs[] >>
+  ‘∃ simp_leaves' . determine_termn_list rec simp_leaves = simp_leaves'’ by gvs[] >>
+  ‘∃ new_edges . mk_new_edges simp_leaves' c = new_edges’ by gvs[] >>
+  ‘∃ new_labels . mk_new_labels simp_leaves' c = new_labels’ by gvs[] >>
+  rgs[] );
 
 
-Definition node_in_BDD_def:
-  node_in_BDD n ((r,edges,labels):('a,'b)BDD) =
-     MEM n (dom_range_edges edges)
-End
+
+val imp_res_tac_body = 
+(imp_res_tac mk_body_map1 >>
+ imp_res_tac mk_body_map2 >>
+ imp_res_tac mk_body_map3 >>
+ imp_res_tac mk_body_map4 >>
+ imp_res_tac mk_body_map5 >>
+ imp_res_tac mk_body_map6);
+
+
+
+
+val imp_res_tac_distinct = 
+(imp_res_tac all_distinct_leaves >>
+ imp_res_tac all_distinct_leaves_labels >>
+ imp_res_tac all_distinct_ntl >>
+ imp_res_tac all_distinct_sub >>
+ imp_res_tac all_distinct_simp >>
+ imp_res_tac all_distinct_determine >>
+ imp_res_tac all_distinct_mk_edges >>
+ imp_res_tac all_distinct_non_term_leaf_updt >>
+ imp_res_tac all_distinct_mk_labels
+);
+
+
 
 
 
@@ -49,6 +83,21 @@ val body_of_mk_pred_tac =
   ‘∃ new_edges . mk_new_edges simp_leaves' c = new_edges’ by gvs[] >>
   ‘∃ new_labels . mk_new_labels simp_leaves' c = new_labels’ by gvs[] >>
   rgs[] );
+
+
+
+
+
+
+
+        
+
+
+ 
+Definition node_in_BDD_def:
+  node_in_BDD n ((r,edges,labels):('a,'b)BDD) =
+     MEM n (dom_range_edges edges)
+End
 
   
 
@@ -65,6 +114,43 @@ Proof
 QED
 
 
+Theorem BDD_sem_determ_not:
+  ∀ n r edges labels mv b rec n' n'' x p.
+    ALOOKUP edges n = SOME (n',n'') ∧
+    ALOOKUP labels n = SOME (non_termn (SOME x,p)) ∧
+    ALOOKUP mv x = SOME T ∧
+    BDD_sem rec (r,edges,labels) mv n b ⇒
+    ~ ∃ b' . b' ≠ b ∧BDD_sem rec (r,edges,labels) mv n b'
+Proof
+ rpt strip_tac >>
+ gvs[Once BDD_sem_cases] >>
+ rgs[Once BDD_sem_cases] >>
+ imp_res_tac BDD_sem_determ
+QED
+
+
+        
+Theorem BDD_sem_not_eq:
+  ∀ n r edges labels mv b rec n' n'' x p b'.
+    ALOOKUP edges n = SOME (n',n'') ∧
+    ALOOKUP labels n = SOME (non_termn (SOME x,p)) ∧
+    ALOOKUP mv x = SOME T ∧
+    BDD_sem rec (r,edges,labels) mv n b ∧
+    ~ BDD_sem rec (r,edges,labels) mv n b' ⇒
+    b' ≠ b
+Proof
+
+ Induct_on ‘BDD_sem’ >>        
+ rpt strip_tac >>
+ rgs[Once BDD_sem_cases] >>
+ gvs[] >>
+
+ rgs[Once BDD_sem_cases] >>
+ gvs[] 
+QED
+
+
+  
   
         
 
@@ -151,8 +237,7 @@ Proof
   ]          
 QED
 
-
-
+         
 
         
 Theorem BDD_sem_exsists:
@@ -207,7 +292,7 @@ Theorem inner_edges_are_same_exists:
     BDD_WF (r',edges',labels') ∧
     body_of_mk rec (r,edges,labels) h c = SOME ((r',edges',labels'),c') ∧
     ALOOKUP edges n = SOME (n',n'') ⇒
-    (∃ n1 n2.ALOOKUP edges' n = SOME (n1,n2) ∧ (n'=n1 ∧ n''=n2))
+    (∃ n1 n2. ALOOKUP edges' n = SOME (n1,n2) ∧ (n'=n1 ∧ n''=n2))
 Proof
   rpt strip_tac >>
   gvs[body_of_mk_def] >>
@@ -286,94 +371,515 @@ gvs[]
 QED
 
 
-(*
-
-mv_dom_bdd mv (r,edges,labels) ∧
-correct_sem rec (r,edges,labels) ∧
-ALOOKUP edges n = SOME (n',n'') ∧
-ALOOKUP labels n = SOME (non_termn (SOME x,p)) ∧
-ALOOKUP edges n' = SOME (n1',n2') ∧
-ALOOKUP labels n' = SOME (non_termn (SOME x',p')) ∧   
-ALOOKUP mv x = SOME T⇒
-rec.sem p' mv = rec.sem p mv
-
-rpt strip_tac >>
-gvs[correct_sem_def] >>
-                     
-first_x_assum (strip_assume_tac o (Q.SPECL [‘n’, ‘mv’, ‘rec.sem p mv’])) >>
-rgs[op_sem_def, get_prop_def]
-   subgoal ‘BDD_sem rec (r,edges,labels) mv n' (rec.sem p mv)’ >-
- (
- simp[Once BDD_sem_cases]
-
- )
+Theorem dom_range_edges_in_append:
+∀ edges new_edges n.
+MEM n (dom_range_edges new_edges) ⇒
+MEM n (dom_range_edges (edges++new_edges))
+Proof
+  Induct >>
+  gvs[dom_range_edges_def]
+QED
 
 
 
-
-
-
-
-
-
-
-
-
-∀ r edges labels r' edges' labels' mv n n' n'' x p c c' b vars_consumed h rec.
-BDD_WF (r,edges,labels) ∧
-BDD_WF (r',edges',labels') ∧
-mv_dom_bdd mv (r',edges',labels') ∧
-consumed_dom_bdd vars_consumed (r,edges,labels) ∧
-correct_sem rec (r,edges,labels) ∧
-body_of_mk rec (r,edges,labels) h c = SOME ((r',edges',labels'),c') ∧
-BDD_sem rec (r',edges',labels') mv n b ∧
-ALOOKUP edges' n = SOME (n',n'') ∧
-ALOOKUP labels' n = SOME (non_termn (SOME x,p)) ∧
-MEM n (dom_range_edges edges') ∧
-ALOOKUP edges n = NONE ⇒
- b = op_sem rec (SOME p) mv
-
-
-rpt strip_tac >>
- rgs[Once BDD_sem_cases] >>
-‘ALOOKUP edges' n' = NONE’ by cheat >>
-   ‘MEM n' (dom_range_edges edges')’ by imp_res_tac lookup_edges_in_domain >>
-
-‘∃ b' p' .is_lookup_ntl labels' n' ∨ ALOOKUP labels' n' = SOME (termn (b',p'))’ by cheat >|[
-    rgs[is_lookup_ntl_def] >>
-    rgs[Once BDD_sem_cases] >>
-    rgs[from_formula_to_action_def] >>
-    rgs[op_sem_def] >>
-
-
-    gvs[body_of_mk_def] >>
+(* when making a new body, the new edges in the new layer indeed has no children *)        
+Theorem mk_body_new_edges_none:
+  ∀r edges labels r' edges' labels' h c c' n n' n'' rec.
+    BDD_WF (r',edges',labels') ∧
+    BDD_WF (r,edges,labels) ∧
+    body_of_mk rec (r,edges,labels) h c = SOME ((r',edges',labels'),c') ∧
+    ALOOKUP edges' n = SOME (n',n'') ∧
+    ALOOKUP edges n = NONE ⇒
+    (ALOOKUP edges' n' = NONE ∧ ALOOKUP edges' n'' = NONE)
+Proof
+  rpt strip_tac >>
+  gvs[body_of_mk_def] >>
   gvs[AllCaseEqs()]>>
-    body_of_mk_pred_tac >>
-
-
-                        
-
-
+  body_of_mk_pred_tac >>
+  
+  
+  ‘ALOOKUP new_edges n = SOME (n',n'')’ by gvs[ALOOKUP_APPEND] >>
+  
+  ‘MEM n (dom_range_edges (edges ++ new_edges))’ by gvs[lookup_edges_in_domain] >>
+  
+  ‘ ∃x p. ALOOKUP (non_term_leaf_updt labels h ⧺ new_labels) n =
+          SOME (non_termn (SOME x,p))’ by
+    (imp_res_tac WF_imp_non_leaf_lbl_abs >>
+     gvs[lookup_is_some_def] >>
+     metis_tac[]) >>
+  
+  simp[ALOOKUP_APPEND] >>
+  simp[AllCaseEqs()]  >|[
+    (* for n' *)
+    ‘MEM n' (MAP FST new_labels)’ by imp_res_tac in_range_of_new_edges_in_dom_new_labels >>
+    ‘MEM n' (dom_range_edges (new_edges))’ by imp_res_tac lookup_edges_in_domain >>
+    ‘MEM n' (dom_range_edges (edges ++ new_edges))’ by gvs[dom_range_edges_in_append] >>
+    Cases_on ‘ALOOKUP (edges ⧺ new_edges) n'’ >|[
+      rgs[ALOOKUP_APPEND] >>
+      rgs[AllCaseEqs()]
+      ,
+      PairCases_on ‘x'’ >>
+      rename1 ‘ALOOKUP (edges ⧺ new_edges) n' = SOME (n1',n2')’ >>
+      subgoal ‘is_lookup_internal (non_term_leaf_updt labels h ⧺ new_labels) n'’ >-
+       (
+       imp_res_tac WF_imp_non_leaf_lbl_abs >>
+       rgs[lookup_is_some_def, is_lookup_internal_def]
+       ) >>
+      
+      rgs[is_lookup_internal_def] >>
+      res_tac >>
+      
+      qpat_x_assum ‘ALOOKUP (non_term_leaf_updt labels h ⧺ new_labels) n' =
+                    SOME (non_termn (SOME x',p'))’ (fn thm => assume_tac (SIMP_RULE (srw_ss()) [ALOOKUP_APPEND] thm)) >>
+      rgs[AllCaseEqs()] >|[
+          ‘ALL_DISTINCT (MAP FST simp_leaves')’ by (rgs[BDD_WF_def] >> imp_res_tac_distinct) >>
+          imp_res_tac new_labels_are_not_internal 
+          ,
+          rgs[BDD_WF_def] >>
+          rgs[ALL_DISTINCT_APPEND] >>
+          imp_res_tac ALOOKUP_MEM >>
+          imp_res_tac mem_fst_snd >>
+          gvs[]
+        ]
+    ]
+                                                
+    ,
+    (* for n'' *)
+    ‘MEM n'' (MAP FST new_labels)’ by imp_res_tac in_range_of_new_edges_in_dom_new_labels >>
+    ‘MEM n'' (dom_range_edges (new_edges))’ by imp_res_tac lookup_edges_in_domain >>
+    ‘MEM n'' (dom_range_edges (edges ++ new_edges))’ by gvs[dom_range_edges_in_append] >>
+    Cases_on ‘ALOOKUP (edges ⧺ new_edges) n''’ >|[
+        rgs[ALOOKUP_APPEND] >>
+        rgs[AllCaseEqs()]
+        ,
+        PairCases_on ‘x'’ >>
+        rename1 ‘ALOOKUP (edges ⧺ new_edges) n'' = SOME (n1',n2')’ >>
+        subgoal ‘is_lookup_internal (non_term_leaf_updt labels h ⧺ new_labels) n''’ >-
+         (
+         imp_res_tac WF_imp_non_leaf_lbl_abs >>
+         rgs[lookup_is_some_def, is_lookup_internal_def]
+         ) >>
+        
+        rgs[is_lookup_internal_def] >>
+        res_tac >>
+        
+        qpat_x_assum ‘ALOOKUP (non_term_leaf_updt labels h ⧺ new_labels) n'' =
+                      SOME (non_termn (SOME x',p'))’
+                     (fn thm => assume_tac (SIMP_RULE (srw_ss()) [ALOOKUP_APPEND] thm)) >>
+        rgs[AllCaseEqs()] >|[
+            ‘ALL_DISTINCT (MAP FST simp_leaves')’ by (rgs[BDD_WF_def] >> imp_res_tac_distinct) >>
+            imp_res_tac new_labels_are_not_internal 
+            ,
+            rgs[BDD_WF_def] >>
+            rgs[ALL_DISTINCT_APPEND] >>
+            imp_res_tac ALOOKUP_MEM >>
+            imp_res_tac mem_fst_snd >>
+            gvs[]
+          ]
+      ]                                       
   ]
-                                                                                     
+QED
 
-                
-Induct_on ‘BDD_sem’ >>
-rpt strip_tac >>
-rgs[]
-gvs[]
 
-res_tac
+
+(* when edges are empty, then root makes a correct BDD *)        
+Theorem edges_empty_correct:
+  ∀r edges labels r' edges' labels' mv n n' n'' x p c c' p' h rec.
+    prop1 rec ∧
+    prop2 rec ∧
+    range_c c ((r,edges,labels):('a,'b) BDD) ∧
+    BDD_WF (r,edges,labels) ∧
+    body_of_mk rec (r,edges,labels) h c = SOME ((r',edges',labels'),c') ∧
+    ALOOKUP edges' n = SOME (n',n'') ∧
+    ALOOKUP labels' n = SOME (non_termn (SOME x,p)) ∧
+    fv_in_labels rec labels mv ∧
+    edges = [] ⇒
+    ((ALOOKUP mv x = SOME T ∧
+      ALOOKUP labels' n' = SOME p' ⇒
+      (from_formula_to_action rec p' mv = op_sem rec (SOME p) mv))
+     ∧
+     (ALOOKUP mv x = SOME F ∧
+      ALOOKUP labels' n'' = SOME p' ⇒
+      (from_formula_to_action rec p' mv = op_sem rec (SOME p) mv)))
+Proof
+  
+  rpt strip_tac >>
+  ‘∃ p' . labels = [(r,p')]’ by gvs[BDD_WF_def] >>
+  gvs[] >>
+  
+  rgs[body_of_mk_def] >>
+  rpt (BasicProvers.FULL_CASE_TAC >> rgs[]) >>
+  
+  rename1 ‘getLeaves [] r' = SOME leaves’ >>
+  rename1 ‘getLabels [(r',p'')] leaves = SOME leaves_labels’ >>
+  rename1 ‘extract_nontermn leaves_labels = SOME ntl’ >>
+  
+  ‘∃ leaves_sub . leaves_pred_sub rec ntl h = leaves_sub’ by gvs[] >>
+  ‘∃ simp_leaves . simp_pred_list rec leaves_sub = simp_leaves’ by gvs[] >>
+  ‘∃ simp_leaves' . determine_termn_list rec simp_leaves = simp_leaves'’ by gvs[] >>
+  ‘∃ new_edges . mk_new_edges simp_leaves' c = new_edges’ by gvs[] >>
+  ‘∃ new_labels . mk_new_labels simp_leaves' c = new_labels’ by gvs[] >>
+  rgs[] >>
+  
+  Cases_on ‘leaves’ >> rgs[getLeaves_def, getLabels_def] >>
+  Cases_on ‘leaves_labels’ >> rgs[] >> PairCases_on ‘h''’ >> rgs[extract_nontermn_def] >>
+  Cases_on ‘h''1’ >> rgs[]  >>
+  
+  rpt (BasicProvers.FULL_CASE_TAC >> gvs[leaves_pred_sub_def]) >>
+  rpt (BasicProvers.FULL_CASE_TAC >> gvs[simp_pred_list_def, mk_new_labels_def]) >>
+  rgs[simp_pred_list_def] >>
+  rgs[leaves_pred_sub_def, determine_termn_def, simp_pred_list_def,
+      determine_termn_list_def, mk_new_edges_def, mk_new_labels_def, non_term_leaf_updt_def,
+      from_formula_to_action_def, op_sem_def] >>
+  rpt (BasicProvers.FULL_CASE_TAC >> gvs[fv_in_labels_def]) >>
+  
+  gvs[BDD_WF_def, range_c_def, dom_range_edges_def] >>
+  
+  
+  gvs[prop2_def] >>
+  res_tac >>
+  gvs[prop1_def] >>
+  res_tac >>
+  gvs[]
+QED
+
+
+    
+
+
+
+
+Theorem leaves_pred_sub_alookup_some:
+  ∀ ntl leaves_sub rec p h n.          
+    ALOOKUP ntl n = SOME p ∧
+    leaves_pred_sub rec ntl h = leaves_sub ⇒
+    ALOOKUP leaves_sub n = SOME (h, rec.sub p h T, rec.sub p h F) 
+Proof
+  Induct >>
+  rpt strip_tac >>
+  imp_res_tac mk_body_map2 >>
+  gvs[leaves_pred_sub_def] >>
+  PairCases_on ‘h’ >> 
+  rgs[AllCaseEqs()] 
+QED
+                                       
+
+
+
+Theorem simp_pred_list_alookup_some:
+  ∀ leaves_sub simp_leaves rec n h pt pf.
+    ALOOKUP leaves_sub n = SOME (h,pt,pf) ∧
+    simp_pred_list rec leaves_sub = simp_leaves ⇒
+    ALOOKUP simp_leaves n = SOME (h, rec.simp pt, rec.simp pf) 
+Proof
+  Induct >>
+  rpt strip_tac >>
+  imp_res_tac mk_body_map3 >>
+  gvs[simp_pred_list_def] >>
+  PairCases_on ‘h’ >> 
+  rgs[AllCaseEqs()] 
+QED
+
+
+Theorem determine_termn_list_alookup_some:
+  ∀ simp_leaves simp_leaves' rec n h ptsimp pfsimp.
+    ALOOKUP simp_leaves n = SOME (h,ptsimp,pfsimp) ∧ 
+    determine_termn_list rec simp_leaves = simp_leaves' ⇒
+    ALOOKUP simp_leaves' n = SOME (h, determine_termn rec ptsimp, determine_termn rec pfsimp) 
+Proof
+  Induct >>
+  rpt strip_tac >>
+  imp_res_tac mk_body_map4 >>
+  gvs[determine_termn_list_def] >>
+  PairCases_on ‘h’ >> 
+  rgs[AllCaseEqs()] 
+QED
+
+
+
+Theorem lookup_new_edges_not_more_than_c:
+  ∀ simp_leaves' c n n' n''.       
+    ALOOKUP (mk_new_edges simp_leaves' c) n = SOME (n',n'') ⇒
+    (n' >= c ∧ n'' >= c)
+Proof
+  Induct >>
+  gvs[mk_new_edges_def] >>
+  rpt strip_tac >>
+  PairCases_on ‘h’ >>
+  gvs[mk_new_edges_def] >>
+  rgs[AllCaseEqs()]  >>
+  res_tac >>
+  gvs[]
+QED
+
+    
 
 
         
 
+                                           
+
+Theorem mk_new_labels_contains_prop:
+  ∀ simp_leaves' new_edges new_labels ptsimp_det pfsimp_det n n' n'' h c.
+    c > n ∧
+    ALOOKUP new_edges n = SOME (n',n'') ∧
+    ALOOKUP simp_leaves' n = SOME (h, ptsimp_det ,  pfsimp_det) ∧
+    mk_new_edges simp_leaves' c = new_edges ∧
+    mk_new_labels simp_leaves' c = new_labels ⇒
+    (ALOOKUP new_labels n' = SOME ptsimp_det ∧
+     ALOOKUP new_labels n'' = SOME pfsimp_det)     
+Proof
+  
+  Induct >>
+  rpt strip_tac >>
+  imp_res_tac mk_body_map5 >-
+   gvs[mk_new_edges_def, mk_new_labels_def, ALOOKUP_def] >-
+   gvs[mk_new_edges_def, mk_new_labels_def, ALOOKUP_def] >>
+
+  imp_res_tac all_distinct_mk_edges >>
+  imp_res_tac all_distinct_mk_labels >>
+  imp_res_tac in_range_of_new_edges_in_dom_new_labels >>
+  
+  PairCases_on ‘h’ >>
+  rgs[AllCaseEqs()] >> 
+  gvs[mk_new_edges_def, mk_new_labels_def] >>
+  
+  imp_res_tac lookup_new_edges_not_more_than_c >>
+  gvs[] >>
+  rgs[AllCaseEqs()] >> 
+  res_tac >>
+  gvs[]                          
+QED
 
 
 
-                        
+
+        
+Theorem body_return_in_decision_str_conv:
+  ∀ simp_leaves' leaves_sub ntl simp_leaves new_edges new_labels n n' n'' p p' p'' h c rec.
+    c > n ∧
+    ALOOKUP ntl n = SOME p ∧
+    ALOOKUP new_edges n = SOME (n',n'') ∧
+    leaves_pred_sub rec ntl h = leaves_sub ∧ 
+    simp_pred_list rec leaves_sub = simp_leaves ∧
+    determine_termn_list rec simp_leaves = simp_leaves' ∧
+    mk_new_edges simp_leaves' c = new_edges ∧
+    mk_new_labels simp_leaves' c = new_labels ⇒
+    ((ALOOKUP new_labels n' = SOME p'
+    ⇒
+    ALOOKUP new_labels n' = SOME (determine_termn rec (rec.simp (rec.sub p h T))))
+     ∧
+     (ALOOKUP new_labels n'' = SOME p''
+      ⇒
+      ALOOKUP new_labels n'' = SOME (determine_termn rec (rec.simp (rec.sub p h F))))
+    )       
+Proof
+  
+  rpt strip_tac >>
+  ‘ALOOKUP leaves_sub n = SOME (h,rec.sub p h T,rec.sub p h F)’ by imp_res_tac leaves_pred_sub_alookup_some >>
+  imp_res_tac simp_pred_list_alookup_some >>
+  ‘ALOOKUP simp_leaves' n =
+   SOME
+   (h,determine_termn rec (rec.simp (rec.sub p h T)),
+    determine_termn rec (rec.simp (rec.sub p h F)))’ by imp_res_tac determine_termn_list_alookup_some >>
+  
+  imp_res_tac mk_new_labels_contains_prop 
+QED
+
+
+
+Theorem statements_structs_correctness_new_layer:
+  ∀ simp_leaves' leaves_sub ntl simp_leaves new_edges new_labels n n' n'' p p' p'' h c mv  rec.        
+    c > n ∧
+    prop1 rec ∧
+    prop2 rec ∧
+    
+    fv_in_p rec p mv ∧
+    ALOOKUP mv h = SOME T ∧
+    
+    ALOOKUP ntl n = SOME p ∧
+    ALOOKUP new_edges n = SOME (n',n'') ∧
+    leaves_pred_sub rec ntl h = leaves_sub ∧ 
+    simp_pred_list rec leaves_sub = simp_leaves ∧
+    determine_termn_list rec simp_leaves = simp_leaves' ∧
+    mk_new_edges simp_leaves' c = new_edges ∧
+    mk_new_labels simp_leaves' c = new_labels ∧
+    ALOOKUP new_labels n' = SOME p'
+    ⇒
+    from_formula_to_action rec p' mv = op_sem rec (SOME p) mv
+Proof
+  
+  rpt strip_tac >>
+  assume_tac  body_return_in_decision_str_conv >>
+  first_x_assum (strip_assume_tac o (Q.SPECL [‘simp_leaves'’, ‘leaves_sub’, ‘ntl’, ‘simp_leaves’, ‘new_edges’, ‘new_labels’, ‘n’,
+                                              ‘n'’, ‘n''’, ‘p’, ‘p'’, ‘p''’, ‘h’, ‘c’, ‘rec’])) >>
+  rgs[] >>
+  
+  rgs[from_formula_to_action_def, op_sem_def] >>
+  rgs[determine_termn_def] >>
+  rgs[AllCaseEqs()]>>
+  rgs[prop1_def] >>
+  rgs[prop2_def] >>
+  res_tac 
+QED
+
+
+
+
+
+
+                                              
+
+
+
+
+                                              
+
+Theorem body_correctness_new_layer:       
+  ∀ r edges labels r' edges' labels' mv n n' n'' x p c c' b vars_consumed h rec.
+    prop1 rec ∧ prop2 rec ∧ range_c c (r,edges,labels) ∧
+          
+    BDD_WF (r,edges,labels) ∧
+    BDD_WF (r',edges',labels') ∧
+    mv_dom_bdd mv (r',edges',labels') ∧
+    fv_in_labels rec labels mv ∧
+    consumed_dom_bdd vars_consumed (r,edges,labels) ∧
+    range_c c (r,edges,labels) ∧
+
+                     
+    correct_sem rec (r,edges,labels) ∧
+    body_of_mk rec (r,edges,labels) h c = SOME ((r',edges',labels'),c') ∧
+    BDD_sem rec (r',edges',labels') mv n b ∧
+    ALOOKUP edges' n = SOME (n',n'') ∧
+    ALOOKUP labels' n = SOME (non_termn (SOME x,p)) ∧
+    ALOOKUP edges n = NONE ⇒
+    b = op_sem rec (SOME p) mv
+Proof
+
+rpt strip_tac >>
+‘ALOOKUP edges' n' = NONE’ by imp_res_tac mk_body_new_edges_none >>
+‘ALOOKUP edges' n'' = NONE’ by imp_res_tac mk_body_new_edges_none >>
+rgs[Once BDD_sem_cases] >>
+rgs[Once BDD_sem_cases] >| [
+    (*case n' *)
+
+    Cases_on ‘MEM n (dom_range_edges edges)’ >|[
+      (* if n is in range of edges, and became in domain of edges' ,
+         then indeed it is a leaf, thus it has been through the body,
+         which entails that that exact n is correct*)
+  
+      gvs[body_of_mk_def] >>
+      gvs[AllCaseEqs()]>>
+      body_of_mk_pred_tac >>
+
+      (*n is in leaves, then indeed in leaves labels *)
+      ‘ALL_DISTINCT (MAP FST edges) ’ by (rgs[BDD_WF_def] >> imp_res_tac_distinct) >>
+      ‘MEM n leaves’ by imp_res_tac leaves_in_get_leaves >>
+      ‘ALOOKUP labels n = SOME (non_termn (NONE,p))’ by  cheat >> (*imp_res_tac lookup_labels_of_leaves_same >>*)
+      ‘x=h’ by  cheat >> (*lookup_non_term_leaf_updt_internal*)
+      rgs[] >>
+
+      ‘ALOOKUP ntl n = SOME p’ by imp_res_tac leaves_in_ntl_lemma >>
+      ‘ALL_DISTINCT (MAP FST labels)’ by cheat >>
+      ‘ALOOKUP leaves_labels n = SOME (non_termn (NONE,p))’ by imp_res_tac leaves_labels_same_in_labels_some >>
+      ‘ALOOKUP new_edges n = SOME (n',n'')’ by cheat >>
+
+      (* we also know that the new label for the new leafs are in new_labels*)
+      ‘ALOOKUP new_labels n' = SOME p'’ by cheat >>
+
+
+      rgs[range_c_def] >>
+
+      assume_tac statements_structs_correctness_new_layer >>
+      first_x_assum (strip_assume_tac o (Q.SPECL [‘simp_leaves'’, ‘leaves_sub’, ‘ntl’, ‘simp_leaves’, ‘new_edges’, ‘new_labels’,
+                                                 ‘n’, ‘n'’, ‘n''’, ‘p’, ‘p'’, ‘p''’, ‘h’, ‘c’, ‘mv’, ‘rec’])) >> 
+      
+
+      subgoal ‘fv_in_p rec p mv’ >-
+       (rgs[fv_in_labels_def] >>
+        metis_tac[]) >>
+        
+      subgoal ‘c > n’ >- (
+       rgs[EVERY_MEM] >>
+       imp_res_tac ALOOKUP_MEM >>
+       imp_res_tac mem_fst_snd >>
+       rgs[]
+      ) >>
+        
+      rgs[]
+               
+      ,
+      (* if n is not in edges, it means either the edges are empty so we work with root, otherwise by contradiction*)
+      Cases_on ‘edges = []’  >|[
+          (* then we should prove the root*)
+          imp_res_tac edges_empty_correct    
+          ,
+          gvs[body_of_mk_def] >>
+          gvs[AllCaseEqs()]>>
+          body_of_mk_pred_tac >>
+                                        
+          imp_res_tac get_leaves_in_nodes >>
+          ‘ALOOKUP leaves_labels n = NONE’ by imp_res_tac not_in_leaves_not_in_res >>
+          subgoal ‘ALOOKUP new_edges n = NONE’ >-
+           (
+           imp_res_tac_body >>
+           rgs[ALOOKUP_NONE] >>
+           imp_res_tac extract_nonterm_mem_neg >>
+           gvs[]
+           ) >>
+              
+           gvs[ALOOKUP_APPEND] >> gvs[]
+        ]
+    ]
+    ,
+    (*case n'' *)
+    cheat
+  ]
+
+
+QED
+
+
                                 
 
+
+
+Theorem bdd_sem_imp:
+  ∀ r edges labels n n' n'' x pred b' rec mv.
+    ALOOKUP edges n = SOME (n',n'') ∧
+    ALOOKUP labels n  = SOME (non_termn (SOME x ,pred)) ∧
+    ALOOKUP mv x = SOME T ∧
+    BDD_sem rec (r,edges,labels) mv n' b' ⇒
+    BDD_sem rec (r,edges,labels) mv n b'
+Proof
+  rpt strip_tac >>
+  simp[Once BDD_sem_cases]
+QED
+
+
+(*
+Prop
+(∃p' x'' b. p = rec.simp (rec.sub p' x'' b))
+
+Theorem WF_imp_non_leaf_lbl_abs_sub_lemma:
+  ∀r edges labels n rec.
+    lookup_is_some edges n ∧
+    BDD_WF (r,edges,labels) ⇒
+    ∃x p x' b. ALOOKUP labels n = SOME (non_termn (SOME x, (rec.simp(rec.sub p x' b))))
+Proof
+  rpt strip_tac >>
+  fs[lookup_is_some_def] >>
+  PairCases_on ‘y’ >>
+  imp_res_tac WF_imp_non_leaf_lbl >>
+  gvs[] >>
+  cheat
+QED  
+*)                                                              
+
+
+                                
+(*** this is lemma 2 (modified) ***)
+Theorem correct_sem_translation_inner_nodes:
   ∀ vars_consumed x r edges labels r' edges' labels' mv n n' n'' h c c' p b rec.                     
     BDD_ordered ((r,edges,labels):('a,'b) BDD) (vars_consumed) ∧
     BDD_WF (r,edges,labels) ∧
@@ -381,7 +887,8 @@ res_tac
              
     mv_dom_bdd mv (r',edges',labels') ∧
     consumed_dom_bdd (vars_consumed) (r,edges,labels) ∧
-                     
+    fv_in_labels rec labels' mv ∧
+                 
     correct_sem rec (r,edges,labels) ∧
     body_of_mk rec (r,edges,labels) h c = SOME ((r',edges',labels'),c') ∧
                
@@ -389,15 +896,13 @@ res_tac
     ALOOKUP edges' n = SOME (n',n'') ∧
     ALOOKUP labels' n = SOME (non_termn (SOME x,p)) ⇒
     b = op_sem rec (SOME p) mv
-
+Proof
 
   ntac 2 strip_tac >>
   measureInduct_on `THE(INDEX_OF x vars_consumed)` >>
   rpt strip_tac >>
-
-   ‘MEM n (dom_range_edges edges')’ by imp_res_tac lookup_edges_in_domain >>
-
-  (*imp_res_tac WFness_range_c_inter >>*)
+  
+  ‘MEM n (dom_range_edges edges')’ by imp_res_tac lookup_edges_in_domain >>
   Cases_on ‘ALOOKUP edges n’ >> rgs[] >|[
     (* this needs the body *)
     cheat
@@ -417,15 +922,9 @@ res_tac
     ‘MEM n2' (dom_range_edges edges)’ by imp_res_tac lookup_edges_in_domain >>
 
     gvs[op_sem_def] >>
-
-
-
-
-                    
-                    
     rgs[Once BDD_sem_cases] >|[
         (*True*)
-        Cases_on ‘ALOOKUP edges n'’ >> rgs[]>|[
+        Cases_on ‘ALOOKUP edges n'’ >> rgs[] >|[
           (* from body *)
           cheat
           ,
@@ -434,19 +933,29 @@ res_tac
                   
           ‘lookup_is_some edges n'’ by gvs[lookup_is_some_def] >>
           ‘∃x p. ALOOKUP labels n' = SOME (non_termn (SOME x,p))’ by (imp_res_tac WF_imp_non_leaf_lbl_abs >> metis_tac[]) >>
-          
-          ‘MEM x' vars_consumed ∧ MEM x vars_consumed’ by (rgs[Once consumed_dom_bdd_def] >> res_tac >> fs[]) >>
-          ‘∃i. INDEX_OF x vars_consumed = SOME i’ by (imp_res_tac MEM_INDEX_OF >> gvs[] )>>
-          ‘∃i'. INDEX_OF x' vars_consumed = SOME i'’ by (imp_res_tac MEM_INDEX_OF >> gvs[]) >>
-
+        
 
           subgoal ‘THE (INDEX_OF x' vars_consumed) < THE (INDEX_OF x vars_consumed)’ >-
            (
+           
+           ‘MEM x' vars_consumed ∧ MEM x vars_consumed’ by (rgs[Once consumed_dom_bdd_def] >> res_tac >> fs[]) >>
+           ‘∃i. INDEX_OF x vars_consumed = SOME i’ by (imp_res_tac MEM_INDEX_OF >> gvs[] )>>
+           ‘∃i'. INDEX_OF x' vars_consumed = SOME i'’ by (imp_res_tac MEM_INDEX_OF >> gvs[]) >>
+           
            rgs[Once BDD_ordered_def]>>
            first_x_assum (strip_assume_tac o (Q.SPECL [‘n’,‘n'’, ‘n''’]))>>
            gvs[order_hold_def]
            ) >>
-          
+
+
+            (*
+        subgoal  ‘∃x p x' b.
+         ALOOKUP labels n' =
+         SOME (non_termn (SOME x,rec.simp (rec.sub p x' b)))’ by (imp_res_tac WF_imp_non_leaf_lbl_abs_sub_lemma >> cheat) >>
+          *)
+
+
+           
                 
           first_x_assum (strip_assume_tac o (Q.SPECL [‘INDEX_OF (x':string) (vars_consumed: string list)’])) >>
           gvs[] >>
@@ -467,28 +976,75 @@ res_tac
           ‘ALOOKUP edges' n' = SOME (n1',n2')’ by (imp_res_tac inner_edges_are_same_exists >> gvs[]) >>
           ‘ALOOKUP labels' n' = SOME (non_termn (SOME x',p'))’ by (imp_res_tac inner_labels_are_same_exists >> gvs[]) >>
           ‘MEM n' (dom_range_edges edges')’ by imp_res_tac lookup_edges_in_domain >>
-          rgs[] >>
+          gvs[] >>
+
+          (****************)
 
 
-          ‘BDD_sem rec (r',edges',labels') mv n b’ by cheat >>
+          gvs[correct_sem_def] >>
 
-          ‘BDD_sem rec (r',edges',labels') mv n' (rec.sem p mv)’ by cheat >>
-          rgs[] >>
-          
-          imp_res_tac BDD_sem_determ >>
-          rgs[Once BDD_sem_cases]
-                                                                                
                 
+
+                
+          subgoal ‘∃b. BDD_sem rec (r,edges,labels) mv n b’ >-
+           (
+           assume_tac BDD_sem_exsists >>
+           first_x_assum (strip_assume_tac o (Q.SPECL [‘(r,edges,labels)’, ‘mv’, ‘n’, ‘vars_consumed’, ‘rec’])) >>
+           gvs[] >>
+           ‘mv_dom_bdd mv (r,edges,labels) ∧ node_in_BDD n (r,edges,labels)’ by cheat >>
+           gvs[] >>
+           srw_tac [SatisfySimps.SATISFY_ss][]
+           ) >>
+
+
+          
+          subgoal ‘∃b. BDD_sem rec (r,edges,labels) mv n' b’ >-
+           (
+           assume_tac BDD_sem_exsists >>
+           first_x_assum (strip_assume_tac o (Q.SPECL [‘(r,edges,labels)’, ‘mv’, ‘n'’, ‘vars_consumed’, ‘rec’])) >>
+           gvs[] >>
+           ‘mv_dom_bdd mv (r,edges,labels) ∧ node_in_BDD n' (r,edges,labels)’ by cheat >>
+           gvs[] >>
+           srw_tac [SatisfySimps.SATISFY_ss][]
+
+           ) >>
+
+
+
+
+           subgoal ‘ b = op_sem rec (get_prop labels n) mv’ >- (
+            first_x_assum (strip_assume_tac o (Q.SPECL [‘n’, ‘mv’, ‘b’])) >>
+            ‘mv_dom_bdd mv (r,edges,labels) ∧ fv_in_labels rec labels mv’ by cheat >>
+            gvs[]
+            ) >>
+          
+          
+          subgoal ‘ b' = op_sem rec (get_prop labels n') mv’ >- (
+            first_x_assum (strip_assume_tac o (Q.SPECL [‘n'’, ‘mv’, ‘b'’])) >>
+            ‘mv_dom_bdd mv (r,edges,labels) ∧ fv_in_labels rec labels mv’ by cheat >>
+            gvs[]
+            ) >>
+
+
+          rgs[get_prop_def] >>
+          rgs[op_sem_def] >>
+
+             qpat_x_assum ‘BDD_sem rec (r,edges,labels) mv n (rec.sem p mv)’
+             (fn thm => assume_tac (SIMP_RULE (srw_ss()) [Once BDD_sem_cases] thm)) >>
+          
+          rgs[] >>
+          imp_res_tac BDD_sem_determ 
           
         ]
         ,
         (* False *)
+        cheat
 
       ]
 
 
   ]
-
+QED
 
                
 
@@ -498,20 +1054,49 @@ res_tac
 
 
 
+
+
+
+
+
+
+
+
+
+
+
+
+
+
+
+
+               
+
+
+
         
 
 Theorem correct_sem_translation_inter:
-  ∀ (BDD:('a,'b) BDD) BDD'' rec c c' vars h vars_consumed  .
-  BDD_ordered BDD'' (h::vars_consumed) ∧      
-  BDD_WF BDD'' ∧
-  consumed_dom_bdd (h::vars_consumed) BDD'' ∧
-  correct_sem rec BDD ∧
-  body_of_mk rec BDD h c = SOME (BDD'',c') ⇒
-  correct_sem rec BDD'' 
-Proof
+  ∀ (BDD:('a,'b) BDD) BDD'' rec c c' vars h vars_consumed.
+    prop1 rec ∧
 
+    range_c c BDD ∧
+    ALL_DISTINCT (h::vars_consumed) ∧
+    BDD_ordered BDD (vars_consumed) ∧      
+    BDD_WF BDD ∧
+    consumed_dom_bdd (vars_consumed) BDD ∧
+                     
+    correct_sem rec BDD ∧
+    body_of_mk rec BDD h c = SOME (BDD'',c') ⇒
+    correct_sem rec BDD'' 
+Proof
   rpt strip_tac >>
-  
+
+
+  imp_res_tac order_translation_inter >>
+  imp_res_tac WFness_range_c_inter >>
+  ‘BDD_WF BDD''’ by imp_res_tac WFness_translation_inter >>
+
   PairCases_on ‘BDD’ >>
   rename1 ‘(r,edges,labels)’ >>
   
@@ -522,6 +1107,7 @@ Proof
   rpt strip_tac >>
 
   Cases_on ‘ALOOKUP edges' n’ >|[
+    (* completly new edges: trivial *)
     rgs[op_sem_def] >>
     rgs[get_prop_def] >>
     rpt (BasicProvers.full_case_tac >> gvs[]) >>
@@ -530,9 +1116,9 @@ Proof
     rgs[from_formula_to_action_def] >>
     Cases_on ‘b’ >> gvs[] >>
   
-    cheat
+    cheat (* TODO: consult with Roberto about this one*)
     ,
-
+    (*inner nodes including the changed layer *)
     Cases_on ‘x’ >>
     rename1 ‘ALOOKUP edges' n = SOME (n',n'')’ >>
 
@@ -544,21 +1130,11 @@ Proof
     rgs[is_lookup_internal_def] >>
     rgs[get_prop_def] >>
 
-    (*************)
-                      
-    rgs[Once BDD_sem_cases] >>
-
-    rgs[op_sem_def]
-    Cases_on ‘b’ >> rgs[] >>
-    rgs[Once BDD_sem_cases] >>
-
-
-    rgs[Once BDD_sem_cases] >>
-    rgs[from_formula_to_action_def] >>
-        rpt (BasicProvers.full_case_tac >> gvs[]) >>
-
-             
-
+    assume_tac correct_sem_translation_inner_nodes >>
+    first_x_assum (strip_assume_tac o (Q.SPECL [‘vars_consumed’, ‘x’, ‘r’, ‘edges’, ‘labels’, ‘r'’,
+                                                ‘edges'’, ‘labels'’, ‘mv’, ‘n’, ‘n'’, ‘n''’, ‘h’, ‘c’,
+                                                ‘c'’])) >>
+    gvs[]
   ]
 
 QED
@@ -566,11 +1142,18 @@ QED
 
 
 
+
+       
+
         
-    
+
+
+        
+                 
 
 Theorem correct_sem_translation:
-  ∀ vars vars_consumed BDD BDD' rec c   .
+  ∀ vars vars_consumed BDD BDD' rec c.
+    prop1 rec ∧
     BDD_ordered BDD vars_consumed ∧
     BDD_WF BDD ∧
     range_c c BDD ∧
@@ -617,8 +1200,6 @@ Proof
     ‘BDD_ordered (r,edges,labels) (h::vars_consumed)’ by cheat >>
     gvs[]>>
                 
-    ‘correct_sem rec (r'',edges'',labels'')’ by cheat >>
-
     ‘ALL_DISTINCT (REVERSE vars ⧺ h::vars_consumed)’ by cheat >>
 
     metis_tac[]
@@ -626,6 +1207,6 @@ Proof
 QED
     
 
-*)
+
 
 val _ = export_theory ();
